lib/haskell_notation.v
@@ -1,14 +1,15 @@
 Require Import lib.utils.
+Require Import ssreflect ssrfun.
 
 (* Monadic function composition *)
 Definition opt_compose {A B C}
                        (f : B -> option C)
                        (g : A -> option B)
                        : A -> option C :=
-  bind f ∘ g.
+  obind f \o g.
 Infix "<=<" := opt_compose (at level 30).
 Arguments opt_compose {A B C} f g / x.
 
 Infix "$"   := (fun f x => f x) (at level 150, left associativity).
 Infix "<$>" := option_map       (at level 130, left associativity).
-Infix "=<<" := bind             (at level 130, left associativity).
+Infix "=<<" := obind            (at level 130, left associativity).
